finish stlc/autosubst2 progress and preservation

stlc/autosubst2/def_extra.v
@@ -1,6 +1,10 @@
+Require Import stlc.autosubst2.prop_as_core.
+Require Import stlc.autosubst2.prop_as_unscoped.
 Require Import stlc.autosubst2.def_as2.
 
 Require Import List.
+Import SubstNotations.
+Import UnscopedNotations.
 
 (* https://github.com/yiyunliu/autosubst-stlc/blob/master/typing.v *)
 
@@ -11,7 +15,7 @@ Inductive lookup {T} : nat -> list T -> T -> Prop :=
 | there n Γ A B : lookup n Γ A -> lookup (S n) (cons B Γ) A.
 
 Reserved Notation "Γ ⊢ t : A" 
-  (at level 50, t at next level, no associativity).
+  (at level 99, t at next level, no associativity).
 Inductive typing : ctx -> exp -> typ -> Prop :=
 | typing_unit : forall (Γ : ctx),
   Γ ⊢ exp_unit : typ_unit
@@ -26,3 +30,19 @@ Inductive typing : ctx -> exp -> typ -> Prop :=
   Γ ⊢ t : A ->
   Γ ⊢ (exp_app s t) : B
 where "Γ ⊢ t : A" := (typing Γ t A).
+
+Reserved Notation "t ⤳ t'" (at level 80).
+Inductive step : exp -> exp -> Prop :=
+| step_beta : forall (t s : exp),
+  exp_app (exp_abs t) s ⤳ t [s..]
+| step_app : forall (t t' s : exp),
+  t ⤳ t' ->
+  exp_app t s ⤳ exp_app t' s
+where "t ⤳ t'" := (step t t').
+
+Definition is_value (t : exp) : Prop :=
+  match t with
+  | exp_abs _ => True
+  | exp_unit => True
+  | _ => False
+  end.
