stlc/autosubst2/prop_typing.v
@@ -1,7 +1,10 @@
 Require Import stlc.autosubst2.prop_as_core.
 Require Import stlc.autosubst2.prop_as_unscoped.
 Require Import stlc.autosubst2.def_as2.
-Require Import stlc.autosubst2.def_typing.
+Require Import stlc.autosubst2.def_extra.
+
+Require Import Coq.Program.Equality.
+Require Import List.
 
 Definition ctx_var_rename {T} ζ Γ Δ :=
   forall i (A : T), lookup i Γ A -> lookup (ζ i) Δ A.
@@ -23,4 +26,65 @@ Proof.
     unfold ctx_var_rename in *. intros.
     inversion H1; subst; asimpl; eauto.
     econstructor. eauto.
+Qed.
+
+Corollary typing_weaken : forall Γ t A B,
+  Γ ⊢ t : A ->
+  (B :: Γ) ⊢ t ⟨↑⟩ : A.
+Proof.
+  intros. 
+  eapply typing_rename; eauto.
+  - unfold ctx_var_rename. intros. eauto.
+Qed.
+
+Definition ctx_var_subst Γ Δ τ := 
+  forall x A, lookup x Γ A -> Δ ⊢ τ x : A.
+
+Theorem typing_subst_var Γ t A : 
+  Γ ⊢ t : A ->
+  forall Δ τ,
+    ctx_var_subst Γ Δ τ ->
+    Δ ⊢ t [τ] : A.
+Proof.
+  intro H. induction H; intros; asimpl; eauto.
+  - eapply typing_abs.
+    eapply IHtyping.
+    unfold ctx_var_subst in *. intros.
+    inversion H1; subst; asimpl; eauto.
+    eapply typing_weaken; eauto.
+Qed.
+
+Corollary typing_subst_var0 Γ t s A B: 
+  (B :: Γ) ⊢ t : A ->
+  Γ ⊢ s : B ->
+  Γ ⊢ t [s..] : A.
+Proof.
+  intros. eapply typing_subst_var; eauto.
+  - unfold ctx_var_subst. intros.
+    inversion H1; subst; asimpl; eauto.
+Qed.
+
+Theorem preservation Γ t t' A : 
+  Γ ⊢ t : A ->
+  t ⤳ t' ->
+  Γ ⊢ t' : A.
+Proof.
+  intros Htyping Hstep. generalize dependent A.
+  induction Hstep; intros; inversion Htyping; subst; eauto.
+  - inversion H2. subst. eauto using typing_subst_var0.
+Qed.
+
+Theorem progress t A : 
+  nil ⊢ t : A ->
+  is_value t \/ exists t', t ⤳ t'.
+Proof.
+  intros H. dependent induction H; simpl; eauto.
+  - inversion H.
+  - right. inversion H; subst.
+    + inversion H1. 
+    + eauto using step. 
+    + specialize (IHtyping1 (JMeq_refl _)).
+      destruct IHtyping1; eauto.
+      * inversion H3.
+      * destruct H3 as [t']. eauto using step.
 Qed.
